examples/WellScopedProof/proof_indp.v
@@ -19,48 +19,6 @@ Lemma lem_ntl1 {A} (n:nat) (t:A) (tl:list A) : In t (n_tl tl n) -> In t tl.
   exact (IHn H0).
 Qed.
 
-(*only used for tProd term, other case is trivial*)
-Lemma term_ind_simpl :
-    forall P : term -> Prop,
-       (forall n : nat, P (tRel n)) ->
-       (forall id : ident, P (tVar id)) ->
-       (forall (ev : nat) (args : list term), P (tEvar ev args)) ->
-       (forall s : sort, P (tSort s)) ->
-       (forall t : term,
-        P t ->
-        forall (kind : cast_kind) (v : term), P v -> P (tCast t kind v)) ->
-      (forall (n : aname) (t : term),
-        P t -> forall t0 : term, P t0 -> P (tProd n t t0)) ->
-       (forall (na : aname) (ty : term),
-        P ty -> forall body : term, P body -> P (tLambda na ty body)) ->
-       (forall (na : aname) (def : term),
-        P def ->
-        forall def_ty : term,
-        P def_ty ->
-        forall body : term, P body -> P (tLetIn na def def_ty body)) ->
-       (forall f : term, P f -> forall args : list term, P (tApp f args)) ->
-       (forall (c : kername) (u : Instance.t), P (tConst c u)) ->
-       (forall (ind : inductive) (u : Instance.t), P (tInd ind u)) ->
-       (forall (ind : inductive) (idx : nat) (u : Instance.t),
-        P (tConstruct ind idx u)) ->
-       (forall (ci : case_info) (type_info : predicate term) (discr : term),
-        P discr ->
-        forall branches : list (branch term),
-        P (tCase ci type_info discr branches)) ->
-       (forall (proj : projection) (t : term), P t -> P (tProj proj t)) ->
-       (forall (mfix : mfixpoint term) (idx : nat), P (tFix mfix idx)) ->
-       (forall (mfix : mfixpoint term) (idx : nat), P (tCoFix mfix idx)) ->
-       (forall i : PrimInt63.int, P (tInt i)) ->
-       (forall f : PrimFloat.float, P (tFloat f)) ->
-       (forall (u : Level.t) (arr : list term) (default : term),
-        P default ->
-        forall type : term, P type -> P (tArray u arr default type)) ->
-       forall t : term, P t.
-Proof.
-  intros.
-  induction t. all:auto.
-Qed.
-
 Lemma lem_aux_nested {n k l ls nind} params narg e t1 :
   has_info l "P" nind ->
   has_info ls "rels_of_T" nind ->
@@ -75,16 +33,15 @@ Proof.
   + intros.
     simpl. destruct (is_rec_call e n) eqn:eq0.
     ++ eapply lem_is_rec_call in eq0. 2:exact H2.
-      apply andb_and. split.
+       eapply lem_tApp.
       - eapply lem_geti_info. exact H2. auto.
         pose (H' := lem_has_info_within2 H0 eq0).
         eapply lem_has_info_within0. exact H'. auto.
-      - apply forallb_Forall. constructor. 2:auto.
-        eapply andb_and. split.
+      - constructor. 2:auto. eapply lem_tApp.
         -- eapply lem_get_info_last. exact H2.
             eapply lem_within_info. auto. auto.
-        -- apply forallb_Forall. eapply lem_rels_of. exact H2.
-    ++ eapply lem_geti_rename. 1:exact H2. simpl in H3.
+        -- eapply lem_rels_of. exact H2.
+    ++ eapply lem_geti_rename. exact H2. simpl in H3.
       apply Compare_dec.leb_complete in H3. auto.
   + intros. inversion H3. apply andb_and in H5. destruct H5.
     change (closedn n0 (
@@ -101,12 +58,11 @@ Proof.
     destruct (is_rec_call e n0) eqn:eq0.
     all : try (eapply (lem_mapt _ _ H2 H3)).
     ++ eapply lem_is_rec_call in eq0. 2:exact H2.
-      apply andb_and. split.
+       eapply lem_tApp.
       - eapply lem_geti_info. exact H2. auto.
         pose (H' := lem_has_info_within2 H0 eq0).
         eapply lem_has_info_within0. exact H'. auto.
-      - apply forallb_Forall. apply Forall_app. split.
-        fold closedn.
+      - apply Forall_app. split.
         eapply Forall_map.
         simpl in H3. apply andb_and in H3. destruct H3.
         eapply forallb_Forall in H4. apply Forall_forall.
@@ -114,10 +70,10 @@ Proof.
         apply lem_ntl1 in H5.
         rewrite Forall_forall in H4. auto.
         fold closedn. constructor. 2:auto.
-        eapply andb_and. split.
+        eapply lem_tApp.
         -- eapply lem_get_info_last. exact H2.
             eapply lem_within_info. auto. auto.
-        -- apply forallb_Forall. eapply lem_rels_of. exact H2.
+        -- eapply lem_rels_of. exact H2.
   Unshelve. all:auto.
 Qed.
 
@@ -138,11 +94,11 @@ Proof.
   + destruct (is_rec_call e n0) eqn:HH.
     ++ eapply lem_mktProd. exact H3. auto. intros.
         eapply lem_kptProd. exact H0.
-        - change (closedn (S n) (geti_info "P" e0 n1) && forallb (closedn (S n)) [get_info_last "args" e0]).
-          apply andb_and. split. eapply lem_geti_info. exact H0. eapply lem_has_info_within1. 2:auto. 2: exact H4.
+        - eapply lem_tApp.
+          eapply lem_geti_info. exact H0. eapply lem_has_info_within1. 2:auto. 2: exact H4.
           eapply (lem_is_rec_call e _ _ H3) in HH.
           eapply (lem_has_info_within2 H4' _).
-          apply forallb_Forall. constructor. 2:auto.
+          constructor. 2:auto.
           eapply lem_get_info_last. exact H0. eapply lem_within_replace.
         - intros. eapply H2. auto.
     ++ eapply lem_kptProd. exact H3.
@@ -166,13 +122,11 @@ Proof.
         -- apply forallb_Forall. apply Forall_map. apply Forall_forall. intros.
           eapply lem_mapt. exact H3. eapply H'. auto.
         -- intros. eapply lem_kptProd. exact H0.
-          +++ change (closedn (S n) (geti_info "P" e0 n1) &&
-              forallb (closedn (S n)) (map (mapt e0) (n_tl args #|params|) ++
-              [get_info_last "args" e0])).
-              apply andb_and. split. eapply lem_geti_info. exact H0. eapply lem_has_info_within1. 3:exact H4. 2:auto.
+          +++ eapply lem_tApp.
+              eapply lem_geti_info. exact H0. eapply lem_has_info_within1. 3:exact H4. 2:auto.
               eapply (lem_is_rec_call e _ _ H3) in eq0.
               eapply (lem_has_info_within2 H4' eq0).
-              apply forallb_Forall. apply app_Forall.
+              apply app_Forall.
               --- apply Forall_map. apply Forall_forall. intros.
                   eapply lem_mapt. exact H0. eapply H'.
                   eapply lem_ntl1. exact H1.
@@ -193,24 +147,19 @@ Lemma lem_transformer_result {n k l ls nind}
 Proof.
   intros.
   unfold transformer_result.
-  change (closedn n (geti_info "P" e i_ind) &&
-    forallb (closedn n)
-      (map (mapt e)
-          (cstrindices) ++
-        [tApp constructor_current
-          (rels_of "params" e ++ rels_of "args" e)])
-  ).
-  apply andb_and. split.
+  eapply lem_tApp.
   + eapply lem_geti_info. exact H1. eapply lem_has_info_within0. 2:exact H2. auto.
-  + apply forallb_Forall. apply app_Forall.
-    ++ apply Forall_map. apply Forall_forall. intros x H8.
+  + apply app_Forall.
+    ++ eapply lem_rels_of. exact H1.
+    ++ apply Forall_app. split. apply Forall_map. apply Forall_forall. intros x H8.
         eapply lem_mapt. exact H1.
         rewrite Forall_forall in H.
         specialize (H x H8). auto.
-    ++ constructor. 2:auto.
-        simpl. apply andb_and. split. auto. apply forallb_Forall. apply app_Forall.
+        constructor. 2:auto.
+        eapply lem_tApp.
+        auto. apply app_Forall.
         - eapply lem_rels_of. exact H1.
-        - eapply lem_rels_of. exact H1.
+        - apply Forall_app. split. eapply lem_rels_of. exact H1. eapply lem_rels_of. exact H1.
 Qed.
 
 Lemma lem_Ffix_args {n k l ls nind} kn params
@@ -251,82 +200,87 @@ Proof.
   inversion H as [_ _ H03]. exact H03. auto.
 Qed.
 
-Lemma lem_Ffix_ctrs' {n k l ls nind} i kn params i_ind b t e:
+Lemma lem_Ffix_ctrs' {n k l ls nind} no_uniform_params i kn params i_ind b t e:
+  Is_closed_context k no_uniform_params ->
   has_info l "P" nind ->
   has_info ls "rels_of_T" nind ->
   i_ind < nind ->
   eprop n k l ls e ->
-  Forall (fun ctor => Is_closed_constructor k ctor) b ->
+  Forall (fun ctor => Is_closed_constructor (k + #|no_uniform_params|) ctor) b ->
   (forall n', forall e', eprop n' k l ls e' -> closedn n' (t e')) ->
-  closedn n (Ffix_ctrs' i kn params i_ind b t e).
+  closedn n (Ffix_ctrs' no_uniform_params i kn params i_ind b t e).
 Proof.
   revert i. revert t. revert n. revert e.
   induction b.
   + simpl. intros.
-    apply H4. auto.
+    eapply H5. exact H3.
   + intros. eapply lem_mktProd.
-    exact H2. eapply lem_auxctr. inversion H3. exact H7.
-    eapply lem_eprop. exact H2. auto. 3:exact H1. auto. auto.
-    intros. fold Ffix_ctrs'. eapply IHb. auto. auto. auto. exact H5. inversion H3. auto.
-    intros. apply H4. auto.
+    exact H3. eapply lemma_it_kptProd. exact H3. auto.
+    intros.
+    eapply lem_auxctr. inversion H4. exact H9.
+    eapply lem_eprop. exact H6. auto. 3:exact H2. auto. auto.
+    intros. fold Ffix_ctrs'. eapply IHb. auto. auto. auto. auto. simpl in H6. auto. inversion H4. auto.
+    intros. eapply H5. exact H7.
 Qed.
 
-Lemma lem_Ffix_bodies_1 {n k l ls} i_ind bodies kn t e:
+Lemma lem_Ffix_bodies_1 {n k l ls} no_uniform_params i_ind bodies kn t e:
+  Is_closed_context k no_uniform_params ->
   (forall n' e', eprop n' k (addl l (Some "P") (i_ind + #|bodies|)) ls e' -> closedn n' (t e')) ->
   eprop n k (addl l (Some "P") i_ind) ls e ->
   Forall
     (fun ind_body =>
-      Is_closed_body k ind_body)
+      Is_closed_body (k + #|no_uniform_params|) ind_body)
     (bodies)
   ->
-  closedn n (Ffix_bodies_1 i_ind bodies kn t e).
+  closedn n (Ffix_bodies_1 no_uniform_params i_ind bodies kn t e).
 Proof.
   revert t. revert i_ind n l. revert e. induction bodies.
-  + intros. simpl. apply H. simpl. simpl in H0.
-    assert (i_ind + 0 = i_ind). auto. rewrite H2.
+  + intros. simpl. apply H0. simpl. simpl in H1.
+    assert (i_ind + 0 = i_ind). auto. rewrite H3.
     auto.
-  + intros. eapply lem_mktProd. exact H0.
-    eapply lemma_it_mktProd. exact H0. inversion H1. inversion H4 as [H40 _ _]. auto.
+  + intros. eapply lem_mktProd. exact H1.
+    eapply lemma_it_kptProd. 2:exact H. exact H1. intros.
+    eapply lemma_it_mktProd. exact H3. inversion H2. inversion H6 as [H60 _ _]. auto.
     intros.
     ++ simpl. apply andb_and. split.
       - apply forallb_Forall. apply app_Forall.
-        -- eapply lem_rels_of. exact H2.
-        -- eapply lem_rels_of. exact H2.
+        -- eapply lem_rels_of. exact H4.
+        -- apply Forall_app. split. eapply lem_rels_of. exact H4.
+           eapply lem_rels_of. exact H4.
       - auto.
     ++ intros.
        fold Ffix_bodies_1.
-      eapply IHbodies.
-      2:exact H2.
-      - intros. apply H.
-        simpl. simpl in H3.
-        assert (S (i_ind + #|bodies|) = i_ind + S #|bodies|). auto.
-        rewrite <- H4. auto.
-      - inversion H1. auto.
+       eapply IHbodies. auto. intros. apply H0.
+       assert (S (i_ind + #|bodies|) = i_ind + S #|bodies|). auto.
+       simpl. rewrite <- H5. exact H4. auto.
+       inversion H2. auto.
 Qed.
 
-Lemma lem_Ffix_bodies_2 {n k l ls nind} i_ind bodies kn params t e:
+Lemma lem_Ffix_bodies_2 {n k l ls nind} no_uniform_params i_ind bodies kn params t e:
+  Is_closed_context k no_uniform_params ->
   has_info l "P" nind ->
   has_info ls "rels_of_T" nind ->
   i_ind + #|bodies| <= nind ->
   eprop n k l ls e ->
   Forall
     (fun ind_body =>
-      Is_closed_body k ind_body)
+      Is_closed_body ( k + #|no_uniform_params|) ind_body)
     (bodies)
   ->
   (forall n', forall e', eprop n' k l ls e' -> closedn n' (t e')) ->
-  closedn n (Ffix_bodies_2 i_ind bodies kn params t e).
+  closedn n (Ffix_bodies_2 no_uniform_params i_ind bodies kn params t e).
 Proof.
   revert n k i_ind t e. induction bodies.
   + simpl. intros.
-    apply H4. auto.
+    apply H5. auto.
   + intros.
     eapply lem_Ffix_ctrs'.
-    2: exact H0. exact H. simpl in H1. lia. exact H2.
-    inversion H3. destruct H7 as [_ H70 _]. exact H70.
-    intros. fold Ffix_bodies_2. eapply IHbodies. auto. auto.
-    simpl in H1. lia.
-    exact H5. inversion H3. auto. auto.
+    2: exact H0. exact H. exact H1. simpl in H2. lia. exact H3.
+    inversion H4. destruct H8 as [_ H80 _]. exact H80.
+    intros. fold Ffix_bodies_2. eapply IHbodies. 2:auto. 2:auto.
+    exact H.
+    simpl in H2. lia.
+    exact H6. inversion H4. auto. auto.
 Qed.
 
 
@@ -336,59 +290,60 @@ Goal forall ty, forall kn,
   closedn 0 (GenerateIndp kn ty).
 Proof.
   intros ty kn H_no_empty H_closed.
+  destruct (SeperateParams kn ty) eqn : eq9.
+  unfold GenerateIndp. rewrite eq9. simpl.
+  pose proof (Hparams := lem_seperateparams kn ty).
+  rewrite eq9 in Hparams.
+  inversion H_closed as [H_closed_params H_closed_body].
+  rewrite Hparams in H_closed_params.
+  pose proof (H_nu_p := lem_is_closed_context3 _ _ _ H_closed_params).
+  pose proof (H_u_p := lem_is_closed_context2 _ _ _ H_closed_params).
   eapply lemma_it_kptProd.
   + eapply lem_initial. auto.
-  + destruct H_closed. auto.
+  + auto.
   + intros e0 H0.
-    eapply lem_Ffix_bodies_1. 2:apply lem_eprop. 2:exact H0.
-    intros. eapply lem_Ffix_bodies_2. 4:exact H.
-    3 : simpl. 3: constructor.
+    rewrite Hparams in H_closed_body.
+    rewrite app_length in H_closed_body.
+    assert (H'' :  (#|ind_bodies ty| + (#|l0| + #|l|)) =
+                    (#|ind_bodies ty| + #|l| + #|l0|) ). lia.
+    rewrite H'' in H_closed_body.
+    eapply lem_Ffix_bodies_1. exact H_nu_p. 2:apply lem_eprop. 2:exact H0.
+    intros. eapply lem_Ffix_bodies_2. 5:exact H.
+    auto.
     simpl. unfold has_info. unfold find. simpl. auto.
-    unfold has_info. simpl. auto.
-    inversion H_closed. auto.
-    intros.
-    ++ eapply lemma_it_mktProd.
-       exact H1. destruct H_closed as [_ H_bodies].
+    unfold has_info. simpl. auto. auto. auto.
+    ++intros.
+      eapply lemma_it_kptProd. 2:exact H_nu_p. exact H1. intros.
+      eapply lemma_it_mktProd.
+       exact H2.
        -unfold no_empty_bodies in H_no_empty.
-        rewrite Forall_forall in H_bodies.
-        specialize (H_bodies (hd todo (ind_bodies ty))).
+        rewrite Forall_forall in H_closed_body.
+        specialize (H_closed_body (hd todo (ind_bodies ty))).
         pose (H' := in_hd todo (ind_bodies ty)).
         specialize (H' H_no_empty).
-        apply H_bodies in H'. inversion H'. auto.
+        apply H_closed_body in H'. inversion H'. auto.
       - intros.
         eapply lem_mktProd.
-        -- exact H2.
-        -- simpl.
-           rewrite <- forallb_Forall.
+        -- exact H3.
+        -- eapply lem_tApp. auto.
            apply app_Forall.
            --- eapply lem_rels_of.
-               exact H2.
-           --- eapply lem_rels_of.
-               exact H2.
-        -- intros.
-          change (
-           closedn
-             (S (n'0 + #|ind_indices (hd todo (ind_bodies ty))|))
-             (rel_of "P" e2)
-           &&
-           forallb
-             (closedn
-               (S (n'0 + #|ind_indices (hd todo (ind_bodies ty))|))
-             ) (rels_of "indices" e2 ++ [rel_of "x" e2])
-         ).
-         apply andb_and.
-         split.
-         --- eapply lem_rel_of.
-             exact H3. simpl.
-             unfold within_info.
-             simpl. auto.
-         --- eapply forallb_Forall.
-             eapply app_Forall.
-             +++ eapply lem_rels_of.
-                 exact H3.
-             +++ constructor. 2:auto.
-                 eapply lem_rel_of.
-                 exact H3. unfold within_info.
-                 simpl. auto.
-    ++ inversion H_closed. auto.
+               exact H3.
+           --- apply Forall_app. split. eapply lem_rels_of. exact H3.
+               eapply lem_rels_of. exact H3.
+        -- intros. eapply lem_tApp.
+            --- eapply lem_geti_info.
+                exact H4. simpl.
+                unfold within_info.
+                simpl. auto.
+            --- eapply app_Forall.
+                +++ eapply lem_rels_of.
+                    exact H4.
+                +++ eapply app_Forall.
+                    eapply lem_rels_of. exact H4.
+                    constructor. 2:auto.
+                    eapply lem_rel_of.
+                    exact H4. unfold within_info.
+                    simpl. auto.
+    ++ auto.
 Qed.
